lib_misc/SteelOptUtils.fst
@@ -1,0 +1,63 @@
+module SteelOptUtils
+
+open Steel.Effect.Atomic
+open Steel.Effect
+open Steel.Reference
+module SM = Steel.Memory
+
+let none_as_emp
+  (#a: Type0)
+  : Pure vprop
+  (requires True)
+  (ensures fun r -> t_of r == option a)
+  =
+  VUnit ({
+    hp = SM.emp;
+    t = option a;
+    sel = fun _ -> None
+  })
+
+let some_as_vp
+  (#a: Type0)
+  (vp: vprop)
+  : Pure vprop
+  (requires t_of vp == a /\ VUnit? vp)
+  (ensures fun r -> t_of r == option a)
+  =
+  VUnit ({
+    hp = hp_of vp;
+    t = option a;
+    sel = fun h -> Some (sel_of vp h)
+  })
+
+
+let c2
+ (#a: Type0)
+ (b: bool)
+ (vp: vprop{t_of vp == a /\ VUnit? vp})
+ : vprop
+ =
+ if b
+ then some_as_vp #a vp
+ else none_as_emp #a
+
+let c2_t
+ (#a: Type0)
+ (b: bool)
+ (vp: vprop{t_of vp == a /\ VUnit? vp})
+ : Lemma
+ (t_of (c2 #a b vp) == option a)
+ = ()
+
+let c2_lemma
+  (#a: Type0)
+  (b: bool)
+  (vp: vprop{t_of vp == a /\ VUnit? vp})
+  (h: hmem (c2 #a b vp))
+  : Lemma
+  (
+    c2_t #a b vp;
+    (b ==> Some? (sel_of (c2 #a b vp) h <: option a)) /\
+    (not b ==> None? (sel_of (c2 #a b vp) h <: option a))
+  )
+  = ()
